\subsection{Power Rule}

Show that
\[%
  \odv{}{x}\left(x^{n}\right) = nx^{n - 1}
.\]%

\begin{proof}
  Using the definition of the derivative, we get the following:
  \[%
    \lim_{h \to 0} \frac{f(a + h) - f(a)}{h}
  .\]%
  We know that $f(x) = x^{n}$. We can expand using the binomial theorem
  \[%
    \lim_{h \to 0} \frac{\displaystyle(a + h)^{n} - a^{n}}{\displaystyle h} = \lim_{h \to 0} \frac{\displaystyle\sum_{k=0}^{n} {n \choose k} a^{k}h^{n - k} - \left(a^{n}\right)}{\displaystyle h}
  .\]%
  After we expand the series, we get the following
  \[%
    \lim_{h \to 0} \frac{\displaystyle\left[{n \choose 0} a^{n}h^{0} + {n \choose 1} a^{n-1}h^{1} + \cdots + {n \choose n-1} a^{1}h^{n-1} + {n \choose n} a^{0}h^{n}\right] - a^{n}}{\displaystyle h}
  ,\]%
  which then, simplifies to
  \[%
    \lim_{h \to 0} \frac{\displaystyle\left[na^{n-1}h + \frac{n(n-1)}{2}a^{n-2}h^{2} + \cdots + h^{n}\right]}{\displaystyle h}
  .\]%
  Each term contains at least one factor of $h$. Using this,
  we can factor and simplify
  \begin{align*}
    &\lim_{h \to 0} \frac{\displaystyle\cancel{h}\left[na^{n-1} + \frac{n(n-1)}{2}a^{n-2}h + \cdots + h^{n-1}\right]}{\cancel{\displaystyle h}} \\
    &= \lim_{h \to 0} \left(na^{n-1} + \frac{n(n-1)}{2}a^{n-2}h + \cdots + h^{n-1} \right) \\
    &= \left(na^{n-1} + \frac{n(n-1)}{2}a^{n-2}0 + \cdots + 0^{n-1}\right) \\
    &= na^{n-1}
  .\end{align*}
  \[%
    \therefore \odv{}{x}\left(x^{n}\right) = nx^{n-1}
  .\]%
\end{proof}
